Add state

nozo/33-IMP-in-Coq/src/IMP.v
@@ -4,6 +4,7 @@ From Coq Require Import Arith.Arith.
 From Coq Require Import Arith.EqNat. Import Nat.
 From Coq Require Import Strings.String.
 
+Module IMP_without_state.
 (* Defining Syntax *)
 
 Inductive aexp : Type :=
@@ -131,3 +132,131 @@ Proof.
         * apply IHa1. reflexivity.
         * apply IHa2. reflexivity.
 Qed.
+End IMP_without_state.
+
+
+
+Module IMP_with_state.
+
+(* Defining state *)
+
+Definition total_map (A : Type) := string -> A.
+
+Definition eqb_string (x y : string) : bool :=
+    if string_dec x y then true else false.
+
+Definition t_empty {A : Type} (v : A) : total_map A :=
+    (fun _ => v).
+
+Definition t_update {A : Type} (m : total_map A)
+                    (x : string) (v : A)
+                    : total_map A :=
+    fun x' => if (eqb_string x x') then v else m x'.
+
+Notation "'_' '!->' v" := (t_empty v)
+    (at level 100, right associativity).
+Notation "x '!->' v ';' m" := (t_update m x v)
+    (at level 100, v at next level, right associativity).
+
+Definition state := total_map nat.
+Definition empty_st := (_ !-> 0).
+Notation "x '!->' v" := (x !-> v ; empty_st)
+    (at level 100).
+
+Definition W : string := "W".
+Definition X : string := "X".
+Definition Y : string := "Y".
+Definition Z : string := "Z".
+
+Compute (X !-> 1; Y !-> 2) X.
+(*
+= 1
+: nat
+ *)
+
+(* Defining Syntax *)
+
+Inductive aexp : Type :=
+    | ANum : nat -> aexp
+    | AId : string -> aexp
+    | APlus : aexp -> aexp -> aexp
+    | AMinus : aexp -> aexp -> aexp
+    | AMult : aexp -> aexp -> aexp.
+
+Inductive bexp : Type :=
+    | BTrue : bexp
+    | BFalse : bexp
+    | BEq : aexp -> aexp -> bexp
+    | BLe : aexp -> aexp -> bexp
+    | BNot : bexp -> bexp
+    | BAnd : bexp -> bexp -> bexp.
+
+(* Defining Notation *)
+
+Coercion AId : string >-> aexp.
+Coercion ANum : nat >-> aexp.
+Declare Custom Entry com.
+Declare Scope com_scope.
+Notation "<{ e }>" := e (at level 0, e custom com at level 99) : com_scope.
+Notation "( x )" := x (in custom com, x at level 99) : com_scope.
+Notation "x" := x (in custom com at level 0, x constr at level 0) : com_scope.
+Notation "f x .. y" := (.. (f x) .. y)
+                  (in custom com at level 0, only parsing,
+                  f constr at level 0, x constr at level 9,
+                  y constr at level 9) : com_scope.
+Notation "x + y" := (APlus x y) (in custom com at level 50, left associativity).
+Notation "x - y" := (AMinus x y) (in custom com at level 50, left associativity).
+Notation "x * y" := (AMult x y) (in custom com at level 40, left associativity).
+Notation "'true'" := true (at level 1).
+Notation "'true'" := BTrue (in custom com at level 0).
+Notation "'false'" := false (at level 1).
+Notation "'false'" := BFalse (in custom com at level 0).
+Notation "x <= y" := (BLe x y) (in custom com at level 70, no associativity).
+Notation "x = y" := (BEq x y) (in custom com at level 70, no associativity).
+Notation "x && y" := (BAnd x y) (in custom com at level 80, left associativity).
+Notation "'~' b" := (BNot b) (in custom com at level 75, right associativity).
+Open Scope com_scope.
+
+Check <{ 3 + (X * 2) }>.
+(* 
+<{ 3 + X * 2 }>
+	 : aexp
+ *)
+
+(* Defining Evaluation as a function *)
+
+Fixpoint aeval (st : state) (a : aexp) : nat :=
+    match a with
+    | ANum n => n
+    | AId x => st x
+    | <{a1 + a2}> => (aeval st a1) + (aeval st a2)
+    | <{a1 - a2}> => (aeval st a1) - (aeval st a2)
+    | <{a1 * a2}> => (aeval st a1) * (aeval st a2)
+    end.
+
+Fixpoint beval (st : state) (b : bexp) : bool :=
+    match b with
+    | <{true}> => true
+    | <{false}> => false
+    | <{a1 = a2}> => (aeval st a1) =? (aeval st a2)
+    | <{a1 <= a2}> => (aeval st a1) <=? (aeval st a2)
+    | <{~ b1}> => negb (beval st b1)
+    | <{b1 && b2}> => andb (beval st b1) (beval st b2)
+    end.
+
+Compute aeval (X !-> 5) <{ 3 + (X * 2) }>.
+(* 
+= 13
+: nat
+ *)
+
+(* Defining Syntax *)
+
+Inductive com : Type :=
+    | CSkip
+    | CAsgn (x : string) (a : aexp)
+    | CSeq (c1 c2 : com)
+    | CIf (b : bexp) (c1 c2 : com) 
+    | CWhile (b : bexp) (c : com).
+
+End IMP_with_state.
